lakefile.lean
@@ -50,4 +50,4 @@ lean_exe interp_tests where
 
 lean_lib Obseq3Proof where
   srcDir := "src"
-  roots := #[`obseq3.proof.common, `obseq3.proof.keystone, `obseq3.proof.permsim_transport, `obseq3.proof.const_write, `obseq3.proof.copy, `obseq3.proof.ref, `obseq3.proof.compiler]
+  roots := #[`obseq3.proof.common, `obseq3.proof.keystone, `obseq3.proof.permsim_transport, `obseq3.proof.spine, `obseq3.proof.const_write, `obseq3.proof.copy, `obseq3.proof.ref, `obseq3.proof.compiler]
